src/Common/Wf.v
@@ -1,0 +1,108 @@
+(** * Miscellaneous Well-Foundedness Facts *)
+Require Import Coq.Setoids.Setoid Coq.Program.Program Coq.Program.Wf Coq.Arith.Wf_nat.
+
+Set Implicit Arguments.
+
+Section wf.
+  Section wf_prod.
+    Context A B (RA : relation A) (RB : relation B).
+
+    Definition prod_relation : relation (A * B)
+      := fun ab a'b' =>
+           RA (fst ab) (fst a'b') \/ (fst a'b' = fst ab /\ RB (snd ab) (snd a'b')).
+
+    Fixpoint well_founded_prod_relation_helper
+             a b
+             (wf_A : Acc RA a) (wf_B : well_founded RB) {struct wf_A}
+    : Acc prod_relation (a, b)
+      := match wf_A with
+           | Acc_intro fa => (fix wf_B_rec b' (wf_B' : Acc RB b') : Acc prod_relation (a, b')
+                              := Acc_intro
+                                   _
+                                   (fun ab =>
+                                      match ab as ab return prod_relation ab (a, b') -> Acc prod_relation ab with
+                                        | (a'', b'') =>
+                                          fun pf =>
+                                            match pf with
+                                              | or_introl pf'
+                                                => @well_founded_prod_relation_helper
+                                                     _ _
+                                                     (fa _ pf')
+                                                     wf_B
+                                              | or_intror (conj pfa pfb)
+                                                => match wf_B' with
+                                                     | Acc_intro fb
+                                                       => eq_rect
+                                                            _
+                                                            (fun a'' => Acc prod_relation (a'', b''))
+                                                            (wf_B_rec _ (fb _ pfb))
+                                                            _
+                                                            pfa
+                                                   end
+                                            end
+                                      end)
+                             ) b (wf_B b)
+         end.
+
+    Definition well_founded_prod_relation : well_founded RA -> well_founded RB -> well_founded prod_relation.
+    Proof.
+      intros wf_A wf_B [a b]; hnf in *.
+      apply well_founded_prod_relation_helper; auto.
+    Defined.
+  End wf_prod.
+
+  Section wf_sig.
+    Context A B (RA : relation A) (RB : forall a : A, relation (B a)).
+
+    Definition sigT_relation : relation (sigT B)
+      := fun ab a'b' =>
+           RA (projT1 ab) (projT1 a'b') \/ (exists pf : projT1 a'b' = projT1 ab, RB (projT2 ab)
+                                                                                    (eq_rect _ B (projT2 a'b') _ pf)).
+
+    Fixpoint well_founded_sigT_relation_helper
+             a b
+             (wf_A : Acc RA a) (wf_B : forall a, well_founded (@RB a)) {struct wf_A}
+    : Acc sigT_relation (existT _ a b).
+    Proof.
+      refine match wf_A with
+               | Acc_intro fa => (fix wf_B_rec b' (wf_B' : Acc (@RB a) b') : Acc sigT_relation (existT _ a b')
+                                  := Acc_intro
+                                       _
+                                       (fun ab =>
+                                          match ab as ab return sigT_relation ab (existT _ a b') -> Acc sigT_relation ab with
+                                            | existT a'' b'' =>
+                                              fun pf =>
+                                                match pf with
+                                                  | or_introl pf'
+                                                    => @well_founded_sigT_relation_helper
+                                                         _ _
+                                                         (fa _ pf')
+                                                         wf_B
+                                                  | or_intror (ex_intro pfa pfb)
+                                                    => match wf_B' with
+                                                         | Acc_intro fb
+                                                           => _(*eq_rect
+                                                            _
+                                                            (fun a'' => Acc sigT_relation (existT B a'' _(*b''*)))
+                                                            (wf_B_rec _ (fb _ _(*pfb*)))
+                                                            _
+                                                            pfa*)
+                                                       end
+                                                end
+                                          end)
+                                 ) b (wf_B a b)
+             end;
+      simpl in *.
+      destruct pfa; simpl in *.
+      exact (wf_B_rec _ (fb _ pfb)).
+    Defined.
+
+    Definition well_founded_sigT_relation : well_founded RA
+                                            -> (forall a, well_founded (@RB a))
+                                            -> well_founded sigT_relation.
+    Proof.
+      intros wf_A wf_B [a b]; hnf in *.
+      apply well_founded_sigT_relation_helper; auto.
+    Defined.
+  End wf_sig.
+End wf.
